Proof of simplified TSan algorithm.

TSan.v
@@ -17,6 +17,939 @@ Section TSan.
   Definition vector_clock := @vector_clock tid.
   Definition operation := @operation tid var lock.
 
+  (* TSan actually corresponds to a slightly different base VC algorithm from
+     FastTrack - one in which reads and writes store their entire VC, rather
+     than just the timestamp of the thread involved. *)
+  Inductive step : @state tid var lock -> operation ->
+    @state tid var lock -> Prop :=
+  | read_upd : forall C L R W t x R' (HW : vc_le (W x) (C t))
+     (HR' : R' = upd R x (vc_join (R x) (C t))),
+     step (C, L, R, W) (rd t x) (C, L, R', W)
+  | write_upd : forall C L R W t x R' W' (HW : vc_le (W x) (C t))
+     (HR : vc_le (R x) (C t)) (HR' : R' = upd R x (C t))
+     (HW : W' = upd W x (C t)),
+     step (C, L, R, W) (wr t x) (C, L, R', W')
+  | acquire : forall C L R W t m C' (HC' : C' = upd C t (vc_join (C t) (L m))),
+     step (C, L, R, W) (acq t m) (C', L, R, W)
+  | release : forall C L R W t m L' C' (HL' : L' = upd L m (C t))
+      (HC' : C' = upd C t (vc_inc t (C t))),
+     step (C, L, R, W) (rel t m) (C', L', R, W)
+  | fork_step : forall C L R W t u C'
+      (HC' : C' = upd (upd C u (vc_join (C u) (C t))) t (vc_inc t (C t))),
+     step (C, L, R, W) (fork t u) (C', L, R, W)
+  | join_step : forall C L R W t u C'
+      (HC' : C' = upd (upd C t (vc_join (C t) (C u))) u (vc_inc u (C u))),
+     step (C, L, R, W) (join t u) (C', L, R, W).
+
+  Definition step_star := rtc step.
+
+  Ltac join_solve := match goal with
+    | [|- vc_join ?a ?b ?c < ?d] => unfold vc_join; apply max_lt; auto
+    | [|- ?d < vc_join ?a ?b ?c] => unfold vc_join; first 
+        [apply lt_max_l; auto | apply lt_max_r; auto]
+    | [|- ?d <= vc_join ?a ?b ?c] => unfold vc_join; first 
+        [apply le_max_l; auto | apply le_max_r; auto]
+    | [|- context[vc_inc ?t ?V ?u]] => unfold vc_inc; destruct (eq_dec u t);
+        clarify; solve [apply Lt.lt_S; auto]
+    end.
+
+  Lemma wf_preservation s s' a (Hwf : well_formed s) (Hstep : step s a s') : 
+    well_formed s'.
+  Proof.
+    destruct s as (((C, L), R), W); 
+      destruct Hwf as [Hthreads [Hlocks [Hread Hwrite]]]; 
+      inversion Hstep; clarify; unfold upd; repeat dec_eq;
+      repeat split; intros; repeat dec_eq; repeat join_solve.
+    - setoid_rewrite Nat.max_lub_iff; clarify.
+      destruct (eq_dec t0 t); clarify.
+      specialize (Hthreads _ _ n); omega.
+    - destruct (eq_dec t0 t); clarify.
+      specialize (Hthreads _ _ n); omega.
+    - destruct (eq_dec t0 t); clarify.
+      specialize (Hthreads _ _ n); omega.
+  Qed.
+
+  Corollary step_star_wf s s' tr (Hwf : well_formed s) 
+    (Hsteps : step_star s tr s') : well_formed s'.
+  Proof.
+    induction Hsteps; auto.
+    apply IHHsteps; eapply wf_preservation; eauto.
+  Qed.
+
+  Lemma clock_mono : forall s s' tr (Hsteps : step_star s tr s') u t,
+    clock_of s u t <= clock_of s' u t.
+  Proof.
+    intros; induction Hsteps; auto.
+    inversion Hstep; unfold upd, vc_inc, vc_join in *; clarify; dec_eq;
+      try omega; eapply Max.max_lub_l; eauto.
+  Qed.
+
+  Lemma lock_no_rel : forall s tr s' m (Hsteps : step_star s tr s')
+    (Hno_rel : Forall (fun a => forall t, a <> rel t m) tr),
+    lock_of s' m = lock_of s m.
+  Proof.
+    intros; induction Hsteps; clarify.
+    inversion Hno_rel as [| ? ? Ha]; clarify.
+    inversion Hstep; clarify.
+    unfold upd in *; clarify.
+    specialize (Ha t); clarify.
+  Qed.
+
+  Lemma feasible_le : forall s tr s' (Hsteps : step_star s tr s') m t t'
+    (Hfeasible : feasible (tr ++ [rel t m])),
+    lock_of s' m t' <= clock_of s' t t'.
+  Proof.
+    intros.
+    inversion Hfeasible; clear Hfeasible Hacq Hfork Hjoin.
+    specialize (Hrel (length tr)); rewrite nth_error_split in Hrel;
+      specialize (Hrel _ _ eq_refl); destruct Hrel as [j Hj].
+    rewrite nth_error_app in Hj; clarify.
+    generalize (nth_error_split' _ _ Hj21); intros [l1 [l2 ?]]; clarify.
+    generalize (rtc_app_inv _ _ Hsteps); intros [s'' Hs'']; clarify.
+    inversion Hs''2 as [| ? ? ? ? Hacq Hsteps'']; clarify.
+    generalize (clock_mono Hsteps'' t t'); clarify.
+    etransitivity; [|eauto].
+    inversion Hacq; unfold upd, vc_join, vc_inc in *; clarify.
+    generalize (lock_no_rel(m := m) Hs''2); intro Heq; clarify; rewrite Heq.
+    apply le_max_r; auto.
+    { constructor; clarify.
+      rewrite Forall_forall; intros ? Hin ?.
+      generalize (in_nth_error _ _ Hin); intros [k Hk].
+      specialize (Hj22 (length l1 + S k)); rewrite app_length in Hj22.
+      use Hj22; [|omega].
+      rewrite <- app_assoc, nth_error_app, lt_dec_plus_r, minus_plus in Hj22;
+        clarify.
+      specialize (Hj22 t0); rewrite nth_error_app, Hk2 in Hj22; intro; clarify.
+    }
+  Qed.
+
+  (* Soundness *)
+  Lemma clocks_hb_core : forall tr s (Hwf : well_formed s) s'
+    (Hsteps : step_star s tr s') t,
+    (forall u, u <> t -> clock_of s t t <= clock_of s' u t ->
+       exists i j e d, nth_error tr i = Some e /\ nth_error tr j = Some d /\
+       uses_thread d u /\ uses_thread e t /\ hbe tr i j) /\
+    (forall m, clock_of s t t <= lock_of s' m t ->
+       exists i j e d, nth_error tr i = Some e /\ nth_error tr j = Some d /\
+       locks d m /\ uses_thread e t /\ hbe tr i j).
+  Proof.
+    induction tr using rev_ind; clarify.
+    { inversion Hsteps; clarify.
+      destruct s' as (((?, ?), ?), ?); destruct Hwf as [Hclock [Hlock _]].
+      split; clarify.
+      - specialize (Hclock u t); clarify; omega.
+      - specialize (Hlock m t); omega. }
+    generalize (rtc_snoc_inv _ _ Hsteps); intros [s'' [Htr Hx]].
+    specialize (IHtr _ Hwf _ Htr t).
+    generalize (step_star_wf Hwf Htr); intro Hwf'.
+    split; [intros ? Ht Hclock | intros ? Hlock]; clarify.
+    - destruct (le_dec (clock_of s t t) (clock_of s'' u t)).
+      { specialize (IHtr1 _ Ht); use IHtr1;
+          destruct IHtr1 as (i & j & ? & ? & Hi & Hj & ?); exists i, j; clarify.
+        generalize (nth_error_lt _ _ Hi), (nth_error_lt _ _ Hj); intros.
+        repeat rewrite nth_error_app; clarify; repeat eexists; eauto.
+        apply hbe_app; auto. }
+      inversion Hx; clarify; unfold upd, vc_join, vc_inc in Hclock; clarify.
+      + generalize (Max.max_spec (C u t) (L m t)); intros [[? Hmax] | [? Hmax]];
+          rewrite Hmax in *; try omega.
+        specialize (IHtr2 _ Hclock).
+        destruct IHtr2 as (i & j & ? & ? & Hi & Hj & ?).
+        generalize (nth_error_lt _ _ Hi), (nth_error_lt _ _ Hj); intros.
+        exists i, (length tr); rewrite nth_error_split; rewrite nth_error_app;
+          unfold uses_thread; clarify; repeat eexists; eauto.
+        eapply hbe_trans; [apply hbe_app; eauto|].
+        left; eapply hb_locking; unfold locks; try (rewrite nth_error_split);
+          try (rewrite nth_error_app); clarify; eauto.
+      + destruct (eq_dec t0 u); clarify.
+        generalize (Max.max_spec (C u t) (C t0 t));
+          intros [[? Hmax] | [? Hmax]]; rewrite Hmax in *; try omega.
+        destruct (eq_dec t0 t); subst.
+        { exists (length tr), (length tr); rewrite nth_error_split;
+            repeat eexists; eauto.
+          * unfold uses_thread, fjs; eauto.
+          * unfold uses_thread; auto.
+          * unfold hbe; auto. }
+        specialize (IHtr1 _ n1); use IHtr1.
+        destruct IHtr1 as (i & j & ? & ? & Hi & Hj & ?); clarify.
+        exists i, (length tr); rewrite nth_error_split.
+        generalize (nth_error_lt _ _ Hi), (nth_error_lt _ _ Hj); intros.
+        rewrite nth_error_app; clarify; repeat eexists; eauto.
+        * unfold uses_thread, fjs; eauto.
+        * eapply hbe_trans; [apply hbe_app; eauto|].
+          left; eapply hb_fork_join; auto; try (rewrite nth_error_split);
+            try (rewrite nth_error_app); clarify; eauto.
+          unfold uses_thread; auto.
+      + destruct (eq_dec u0 u); clarify.
+        generalize (Max.max_spec (C u t) (C u0 t));
+          intros [[? Hmax] | [? Hmax]]; rewrite Hmax in *; try omega.
+        destruct (eq_dec u0 t); subst.
+        { exists (length tr), (length tr); rewrite nth_error_split;
+            repeat eexists; eauto.
+          * unfold uses_thread; auto.
+          * unfold uses_thread, fjs; eauto.
+          * unfold hbe; auto. }
+        specialize (IHtr1 _ n1); use IHtr1.
+        destruct IHtr1 as (i & j & ? & ? & Hi & Hj & ?); clarify.
+        exists i, (length tr); rewrite nth_error_split.
+        generalize (nth_error_lt _ _ Hi), (nth_error_lt _ _ Hj); intros.
+        rewrite nth_error_app; clarify; repeat eexists; eauto.
+        * unfold uses_thread, fjs; eauto.
+        * eapply hbe_trans; [apply hbe_app; eauto|].
+          left; eapply hb_fork_join; auto; try (rewrite nth_error_split);
+            try (rewrite nth_error_app); clarify; eauto.
+          unfold uses_thread, fjs; eauto.
+    - destruct (le_dec (clock_of s t t) (lock_of s'' m t)).
+      { specialize (IHtr2 m); use IHtr2;
+          destruct IHtr2 as (i & j & ? & ? & Hi & Hj & ?); exists i, j; clarify.
+        generalize (nth_error_lt _ _ Hi), (nth_error_lt _ _ Hj); intros.
+        unfold locks in *; clarify.
+        repeat rewrite nth_error_app; clarify; repeat eexists; eauto.
+        apply hbe_app; auto. }
+      inversion Hx; clarify; unfold upd, vc_join, vc_inc in Hlock; clarify.
+      destruct (eq_dec t0 t); subst.
+      + exists (length tr), (length tr); rewrite nth_error_split;
+          repeat eexists; eauto.
+        * unfold uses_thread; auto.
+        * unfold hbe; auto.
+      + specialize (IHtr1 _ n0); use IHtr1.
+        destruct IHtr1 as (i & j & ? & ? & Hi & Hj & ?); clarify.
+        exists i, (length tr); rewrite nth_error_split.
+        generalize (nth_error_lt _ _ Hi), (nth_error_lt _ _ Hj); intros.
+        rewrite nth_error_app; clarify; repeat eexists; eauto.
+        eapply hbe_trans; [apply hbe_app; eauto|].
+        left; eapply hb_fork_join; auto; try (rewrite nth_error_split);
+          try (rewrite nth_error_app); clarify; eauto.
+        unfold uses_thread; auto.
+  Qed.
+  (* This seems to be the core of the relationship between vector clocks and
+     the happens-before order. Does it appear in the literature? *)
+
+  Lemma clocks_hb sa a tr sb b : forall (Hwf : well_formed sa)
+    (Hsteps : step_star sa (a :: tr) sb)
+    t (Ht : t = thread_of a) u (Hu : u = thread_of b)
+    (Hclock_lt : clock_of sa t t <= clock_of sb u t),
+    happens_before (a :: tr ++ [b]) 0 (S (length tr)).
+  Proof.
+    intros.
+    destruct (eq_dec u t).
+    - subst; symmetry in e; eapply hb_prog_order; eauto; clarify.
+      apply nth_error_split.
+    - generalize (clocks_hb_core Hwf Hsteps t); intros [Hhb _].
+      specialize (Hhb _ n Hclock_lt).
+      destruct Hhb as (i & j & e & d & Hi & Hj & ?); clarify.
+      generalize (nth_error_lt _ _ Hi), (nth_error_lt _ _ Hj); intros.
+      eapply hbe_hb_trans; [|eapply hbe_hb_trans].
+      + unfold hbe; destruct (eq_dec 0 i); eauto.
+        left; eapply hb_fork_join; clarify; eauto.
+        * omega.
+        * destruct i; clarify; rewrite nth_error_app; clarify; omega.
+        * unfold uses_thread; auto.
+      + assert (hbe ((a :: tr) ++ [b]) i j) by (apply hbe_app; auto);
+          clarify; eauto.
+      + eapply hb_fork_join; clarify.
+        * instantiate (1 := d); destruct j; clarify.
+          rewrite <- Nat.succ_lt_mono, nth_error_app in *; clarify.
+        * apply nth_error_split.
+        * eauto.
+        * unfold uses_thread; auto.
+  Qed.
+
+  Lemma clocks_hb' tr1 sa a tr2 sb b tr3 : forall (Hwf : well_formed sa)
+    (Hsteps : step_star sa (a :: tr2) sb)
+    t (Ht : t = thread_of a) u (Hu : u = thread_of b)
+    (Hclock_lt : clock_of sa t t <= clock_of sb u t),
+    happens_before (tr1 ++ a :: tr2 ++ b :: tr3)
+                   (length tr1) (length tr1 + S (length tr2)).
+  Proof.
+    intros; generalize (clocks_hb _ Hwf Hsteps Ht Hu Hclock_lt); intro Hhb.
+    generalize (hb_app tr3 (hb_app' tr1 Hhb)); clarsimp.
+  Qed.
+
+  Lemma write_own' : forall tr s x t (Hsteps : step_star s0 tr s)
+    (Hwrite : write_of s x t = clock_of s t t),
+    vc_le (write_of s x) (clock_of s t) /\ vc_le (read_of s x) (clock_of s t).
+  Proof.
+    induction tr using rev_ind; clarify.
+    { inversion Hsteps; split; intro; clarify. }
+    generalize (rtc_snoc_inv _ _ Hsteps); intros [s' [Htr Hs']].
+    generalize (step_star_wf wf0 Htr); intro Hwf.
+    specialize (IHtr _ x0 t Htr).
+    inversion Hs'; clarify.
+    - unfold upd in *; clarify.
+      intro; clarify.
+      setoid_rewrite Nat.max_lub_iff; clarify.
+      destruct (eq_dec t t0); clarify.
+      specialize (Hwf1 _ _ n); specialize (HW t).
+      destruct (eq_dec t1 t); clarify; omega.
+    - unfold upd in *; clarify.
+      destruct (eq_dec t t0); [split; intro|]; clarify.
+      specialize (Hwf1 _ _ n); omega.
+    - unfold upd in *; clarify.
+      unfold vc_join in Hwrite; rewrite Max.max_l in Hwrite; clarify.
+      split; intro; join_solve.
+      { specialize (Hwf21 m t); omega. }
+    - unfold upd, vc_inc in *; clarify.
+      specialize (Hwf222 x0 t); omega.
+    - unfold upd, vc_inc in *; clarify.
+      destruct (eq_dec t0 t); clarify.
+      + specialize (Hwf222 x0 t); omega.
+      + unfold vc_join in Hwrite; rewrite Max.max_l in Hwrite; clarify.
+        split; intro; join_solve.
+        { specialize (Hwf1 t0 t); clarify; omega. }
+    - unfold upd, vc_inc in *; clarify.
+      destruct (eq_dec u t); clarify.
+      + specialize (Hwf222 x0 t); omega.
+      + unfold vc_join in Hwrite; rewrite Max.max_l in Hwrite; clarify.
+        split; intro; join_solve.
+        { specialize (Hwf1 u t); clarify; omega. }
+  Qed.
+
+  Corollary write_own : forall tr s x t (Hsteps : step_star s0 tr s)
+    (Hwrite : write_of s x t = clock_of s t t),
+    vc_le (write_of s x) (clock_of s t).
+  Proof. apply write_own'. Qed.
+
+  Lemma write_mono : forall s tr s' x (Hsteps : step_star s tr s'),
+    vc_le (write_of s x) (write_of s' x).
+  Proof.
+    intros; induction Hsteps; intro; clarify.
+    etransitivity; [|eapply IHHsteps].
+    inversion Hstep; clarify.
+    unfold upd; clarify.
+  Qed.
+
+  Lemma read_mono : forall s tr s' x (Hsteps : step_star s tr s')
+    (Hwf : well_formed s), vc_le (read_of s x) (read_of s' x).
+  Proof.
+    intros; induction Hsteps; intro; clarify.
+    generalize (wf_preservation Hwf Hstep); intro.
+    etransitivity; [|apply IHHsteps; auto].
+    inversion Hstep; clarify; unfold upd; clarify.
+    apply Max.le_max_l.
+  Qed.
+
+  Lemma write_result : forall s t x s' (Hstep : step s (wr t x) s'),
+    write_of s' x t = clock_of s t t /\ clock_of s' t = clock_of s t.
+  Proof.
+    intros; inversion Hstep; unfold upd in *; clarify.
+  Qed.
+
+  Lemma write_after_write : forall tr s i j x t u
+    (Hsteps : step_star s0 tr s) (Hlt : i < j)
+    (Hi : nth_error tr i = Some (wr t x)) (Hj : nth_error tr j = Some (wr u x)),
+     happens_before tr i j.
+  Proof.
+    intros.
+    assert (tr = firstn i tr ++ wr t x :: firstn (j - S i) (skipn (S i) tr) ++
+      wr u x :: skipn (S j) tr) as Htr.
+    { rewrite <- (firstn_skipn i tr) at 1; erewrite skipn_n; eauto.
+      rewrite <- (firstn_skipn (j - S i) (skipn (S i) tr)) at 1.
+      rewrite skipn_skipn, le_plus_minus_r; [|auto].
+      erewrite (skipn_n j); eauto. }
+    generalize (nth_error_lt _ _ Hi), (nth_error_lt _ _ Hj); intros.
+    assert (i = length (firstn i tr)) as Hi'.
+    { rewrite List.firstn_length, Min.min_l; auto; omega. }
+    assert (j = length (firstn i tr) + S (length (firstn (j - S i)
+      (skipn (S i) tr)))) as Hj'.
+    { repeat rewrite List.firstn_length; rewrite skipn_length.
+      repeat rewrite Min.min_l; omega. }
+    rewrite Hi', Hj'; rewrite Htr at 1; clear Hi' Hj'.
+    rewrite Htr in Hsteps; clear Htr.
+    generalize (rtc_app_inv _ _ Hsteps); intros (? & ? & Hsteps').
+    rewrite app_comm_cons in Hsteps'; generalize (rtc_app_inv _ _ Hsteps');
+      intros (? & Hstepsi & Hstepsj).
+    eapply clocks_hb'; eauto.
+    { eapply step_star_wf; eauto; apply wf0. }
+    inversion Hstepsi as [|? ? ? ? Hstepi Htr2]; clarify.
+    inversion Hstepsj as [|? ? ? ? Hstepj ?]; clarify.
+    generalize (write_result Hstepi), (write_result Hstepj);
+      intros [Hwi Hci] [Hwj Hcj].
+    rewrite <- Hcj in *; etransitivity; [|eapply write_own; eauto].
+    generalize (rtc_snoc _ _ Htr2 Hstepj); intro.
+    etransitivity; [|eapply write_mono; eauto]; clarsimp.
+    { eapply rtc_snoc; [|eauto].
+      eapply rtc_trans; eauto. }
+  Qed.
+
+  Lemma read_own : forall tr s x t (Hsteps : step_star s0 tr s)
+    (Hwrite : read_of s x t = clock_of s t t),
+    vc_le (write_of s x) (clock_of s t).
+  Proof.
+    induction tr using rev_ind; clarify.
+    { inversion Hsteps; intro; clarify. }
+    generalize (rtc_snoc_inv _ _ Hsteps); intros [s' [Htr Hs']].
+    generalize (step_star_wf wf0 Htr); intro Hwf.
+    specialize (IHtr _ x0 t Htr).
+    inversion Hs'; clarify.
+    - unfold upd in *; clarify.
+      destruct (eq_dec t t0); clarify.
+      specialize (Hwf1 _ _ n).
+      generalize (Max.max_spec (R x0 t) (C t0 t)); intros [[? Hmax] | [? Hmax]];
+        setoid_rewrite Hmax in Hwrite; [omega | clarify].
+    - unfold upd in *; clarify.
+      intro; clarify.
+      destruct (eq_dec t t0); clarify.
+      specialize (Hwf1 _ _ n); specialize (HR t); omega.
+    - unfold upd in *; clarify.
+      unfold vc_join in Hwrite; rewrite Max.max_l in Hwrite; clarify.
+      intro; join_solve.
+      { specialize (Hwf21 m t); omega. }
+    - unfold upd, vc_inc in *; clarify.
+      specialize (Hwf221 x0 t); omega.
+    - unfold upd, vc_inc in *; clarify.
+      destruct (eq_dec t0 t); clarify.
+      + specialize (Hwf221 x0 t); omega.
+      + unfold vc_join in Hwrite; rewrite Max.max_l in Hwrite; clarify.
+        intro; join_solve.
+        { specialize (Hwf1 t0 t); clarify; omega. }
+    - unfold upd, vc_inc in *; clarify.
+      destruct (eq_dec u t); clarify.
+      + specialize (Hwf221 x0 t); omega.
+      + unfold vc_join in Hwrite; rewrite Max.max_l in Hwrite; clarify.
+        intro; join_solve.
+        { specialize (Hwf1 u t); clarify; omega. }
+  Qed.
+  
+  Lemma read_result : forall s t x s' (Hstep : step s (rd t x) s')
+    (Hwf : well_formed s),
+    read_of s' x t = clock_of s t t /\ clock_of s' t = clock_of s t.
+  Proof.
+    intros; inversion Hstep; unfold upd in *; clarify.
+    setoid_rewrite Max.max_r; auto.
+  Qed.
+
+  Lemma read_after_write : forall tr s i j x t u
+    (Hsteps : step_star s0 tr s) (Hlt : i < j)
+    (Hi : nth_error tr i = Some (wr t x)) (Hj : nth_error tr j = Some (rd u x)),
+    happens_before tr i j.
+  Proof.
+    intros.
+    assert (tr = firstn i tr ++ wr t x :: firstn (j - S i) (skipn (S i) tr) ++
+      rd u x :: skipn (S j) tr) as Htr.
+    { rewrite <- (firstn_skipn i tr) at 1; erewrite skipn_n; eauto.
+      rewrite <- (firstn_skipn (j - S i) (skipn (S i) tr)) at 1.
+      rewrite skipn_skipn, le_plus_minus_r; [|auto].
+      erewrite (skipn_n j); eauto. }
+    generalize (nth_error_lt _ _ Hi), (nth_error_lt _ _ Hj); intros.
+    assert (i = length (firstn i tr)) as Hi'.
+    { rewrite List.firstn_length, Min.min_l; auto; omega. }
+    assert (j = length (firstn i tr) + S (length (firstn (j - S i)
+      (skipn (S i) tr)))) as Hj'.
+    { repeat rewrite List.firstn_length; rewrite skipn_length.
+      repeat rewrite Min.min_l; omega. }
+    rewrite Hi', Hj'; rewrite Htr at 1; clear Hi' Hj'.
+    rewrite Htr in Hsteps; clear Htr.
+    generalize (rtc_app_inv _ _ Hsteps); intros (? & ? & Hsteps').
+    rewrite app_comm_cons in Hsteps'; generalize (rtc_app_inv _ _ Hsteps');
+      intros (? & Hstepsi & Hstepsj).
+    eapply clocks_hb'; eauto.
+    { eapply step_star_wf; eauto; apply wf0. }
+    inversion Hstepsi as [|? ? ? ? Hstepi Htr2]; clarify.
+    inversion Hstepsj as [|? ? ? ? Hstepj ?]; clarify.
+    generalize (step_star_wf wf0 H1); intro Hwf0.
+    exploit step_star_wf; eauto; intro Hwf1.
+    generalize (write_result Hstepi), (read_result Hstepj Hwf1);
+      intros [Hwi Hci] [Hwj Hcj].
+    rewrite <- Hcj in *; etransitivity; [|eapply read_own; eauto].
+    generalize (rtc_snoc _ _ Htr2 Hstepj); intro.
+    etransitivity; [|eapply write_mono; eauto]; clarsimp.
+    { eapply rtc_snoc; [|eauto].
+      eapply rtc_trans; eauto. }
+  Qed.
+
+  Lemma write_after_read : forall tr s i j x t u
+    (Hsteps : step_star s0 tr s) (Hlt : i < j)
+    (Hi : nth_error tr i = Some (rd t x)) (Hj : nth_error tr j = Some (wr u x)),
+    happens_before tr i j.
+  Proof.
+    intros.
+    assert (tr = firstn i tr ++ rd t x :: firstn (j - S i) (skipn (S i) tr) ++
+      wr u x :: skipn (S j) tr) as Htr.
+    { rewrite <- (firstn_skipn i tr) at 1; erewrite skipn_n; eauto.
+      rewrite <- (firstn_skipn (j - S i) (skipn (S i) tr)) at 1.
+      rewrite skipn_skipn, le_plus_minus_r; [|auto].
+      erewrite (skipn_n j); eauto. }
+    generalize (nth_error_lt _ _ Hi), (nth_error_lt _ _ Hj); intros.
+    assert (i = length (firstn i tr)) as Hi'.
+    { rewrite List.firstn_length, Min.min_l; auto; omega. }
+    assert (j = length (firstn i tr) + S (length (firstn (j - S i)
+      (skipn (S i) tr)))) as Hj'.
+    { repeat rewrite List.firstn_length; rewrite skipn_length.
+      repeat rewrite Min.min_l; omega. }
+    rewrite Hi', Hj'; rewrite Htr at 1; clear Hi' Hj'.
+    rewrite Htr in Hsteps; clear Htr.
+    generalize (rtc_app_inv _ _ Hsteps); intros (? & ? & Hsteps').
+    rewrite app_comm_cons in Hsteps'; generalize (rtc_app_inv _ _ Hsteps');
+      intros (? & Hstepsi & Hstepsj).
+    eapply clocks_hb'; eauto.
+    { eapply step_star_wf; eauto; apply wf0. }
+    inversion Hstepsi as [|? ? ? ? Hstepi Htr2]; clarify.
+    inversion Hstepsj as [|? ? ? ? Hstepj ?]; clarify.
+    generalize (step_star_wf wf0 H1); intro Hwf0.
+    generalize (read_result Hstepi Hwf0), (write_result Hstepj);
+      intros [Hwi Hci] [Hwj Hcj].
+    rewrite <- Hcj in *; etransitivity; [|eapply write_own'; eauto].
+    generalize (rtc_snoc _ _ Htr2 Hstepj); intro.
+    etransitivity; [|eapply read_mono; eauto]; clarsimp.
+    { eapply (step_star_wf wf0).
+      eapply rtc_snoc; eauto. }
+    { eapply rtc_snoc; [|eauto].
+      eapply rtc_trans; eauto. }
+  Qed.
+
+  Theorem Soundness tr : forall s', step_star s0 tr s' -> race_free tr.
+  Proof.
+    intros; rewrite race_free_alt; repeat intro; clarify.
+    unfold writes in *; destruct Haccesses1 as [t [H1 | H1]],
+      Haccesses2 as [u [H2 | H2]]; clarify.
+    - eapply write_after_read; eauto.
+    - eapply read_after_write; eauto.
+    - eapply write_after_write; eauto.
+  Qed.
+
+  Lemma K_upper : forall a s s' (Hstep : step s a s') t t',
+    K a s t t' <= clock_of s' t t'.
+  Proof.
+    intros.
+    generalize (clock_mono (ss_step _ _ Hstep (ss_refl _ _)) t t'); intro.
+    destruct a; clarify; inversion Hstep; clarify.
+  Qed.
+
+  Lemma acq_rel_clock : forall s t m tr s'
+    (Hsteps : step_star s (acq t m :: tr ++ [rel t m]) s'),
+    vc_le (clock_of s t) (lock_of s' m).
+  Proof.
+    intros.
+    inversion Hsteps as [|? ? ? ? Ha Htr]; clarify.
+    inversion Ha; clarify.
+    generalize (rtc_snoc_inv _ _ Htr); intros [s'' [Htr' Hx]].
+    inversion Hx; clarify.
+    unfold upd; clarify.
+    generalize (ss_step _ _ Ha Htr'); intro Hsteps'.
+    generalize (clock_mono Hsteps'); unfold vc_le; auto.
+  Qed.
+
+  Lemma lock_mono : forall s tr s' tr' s'' (Hsteps : step_star s tr s')
+    (Hsteps' : step_star s' tr' s'') m t (Hfeasible : feasible (tr ++ tr')),
+    lock_of s' m t <= lock_of s'' m t.
+  Proof.
+    induction tr' using rev_ind; clarify.
+    { inversion Hsteps'; clarify. }
+    generalize (rtc_snoc_inv _ _ Hsteps'); intros [sx [Htr' Hx]].
+    specialize (IHtr' _ Hsteps Htr' m t).
+    rewrite app_assoc in Hfeasible; generalize (feasible_snoc _ _ Hfeasible);
+      clarify.
+    inversion Hx; unfold upd, vc_inc, vc_join in *; clarify.
+    generalize (rtc_trans Hsteps Htr'); intro Htr.
+    generalize (feasible_le Htr m t0 t Hfeasible); clarify; omega.
+  Qed.
+
+  Lemma hb_clocks : forall s tr1 sa (Hsteps1 : step_star s tr1 sa)
+    a sa' (Hstepa : step sa a sa') tr2 sb (Hsteps2 : step_star sa' tr2 sb)
+    b t (Ht : t = thread_of a) u (Hu : u = thread_of b) tr3
+    (Hhb : happens_before (tr1 ++ a :: tr2 ++ b :: tr3) (length tr1) 
+             (length tr1 + S (length tr2)))
+    (Hfeasible : feasible (tr1 ++ a :: tr2 ++ b :: tr3)),
+    vc_le (K a sa t) (K b sb u).
+  Proof.
+    repeat intro.
+    destruct (eq_dec t u).
+    { rewrite e; etransitivity; [apply K_upper; eauto|].
+      etransitivity; [|apply K_lower].
+      eapply clock_mono; eauto. }
+    remember (length tr1 + S (length tr2)) as j; remember (length tr1) as i;
+      remember (tr1 ++ a :: tr2 ++ b :: tr3) as tr.
+    generalize dependent tr1; generalize dependent tr2;
+      generalize dependent tr3; generalize dependent a; generalize dependent b;
+      generalize dependent u; revert sa sa' sb t.
+    induction Hhb; clarify.
+    - rewrite nth_error_split in Ha; clarify.
+      rewrite nth_error_app, lt_dec_plus_r, minus_plus in Hb; clarify.
+      rewrite nth_error_split in Hb; clarify.
+    - rewrite nth_error_split in Ha; clarify.
+      rewrite nth_error_app, lt_dec_plus_r, minus_plus in Hb; clarify.
+      rewrite nth_error_split in Hb; clarify.
+      (* Consider: given feasible, this reduces to the case in which
+         a releases and b acquires. *)
+      destruct Hlocka as [t Hlocka], Hlockb as [u Hlockb].
+      assert (exists l1 sr sr' l2 sc l3, a :: tr2 ++ [b] = l1 ++ rel t m :: l2
+        ++ acq u m :: l3 /\ step_star sa l1 sr /\ step sr (rel t m) sr' /\
+        step_star sr' l2 sc /\
+        (l3 = [] /\ sc = sb \/ step_star sc (acq u m :: removelast l3) sb))
+        as (l1 & sr & sr' & l2 & sc & l3 & Hra).
+      { inversion Hfeasible; clear Hfork Hjoin.
+        destruct Hlockb; clarify.
+        + destruct Hlocka; clarify.
+          * specialize (Hacq (length tr1 + S (length tr2))).
+            rewrite nth_error_app, lt_dec_plus_r, minus_plus in Hacq;
+              simpl in Hacq; rewrite nth_error_split in Hacq.
+            specialize (Hacq _ _ eq_refl (length tr1) t);
+              rewrite nth_error_split in Hacq; use Hacq; use Hacq.
+            destruct Hacq as [k Hk]; clarify.
+            rewrite nth_error_app in Hk2; destruct (lt_dec k (length tr1));
+              [omega|].
+            destruct (k - length tr1) eqn: Hminus; clarify.
+            rewrite nth_error_app in Hk2; destruct (lt_dec n1 (length tr2));
+              [|omega].
+            generalize (nth_error_split' _ _ Hk2); intros [l1 [l2 ?]];
+              clarify.
+            generalize (rtc_app_inv _ _ Hsteps2); intros [sr [? Hsr]].
+            inversion Hsr; clarify.
+            exists (acq t m :: l1), sr, s', l2, sb, []; clarsimp.
+            econstructor; eauto.
+          * exists [], sa, sa', tr2, sb, []; clarify; apply ss_refl.
+        + specialize (Hrel (length tr1 + S (length tr2))).
+          rewrite nth_error_app, lt_dec_plus_r, minus_plus in Hrel;
+            simpl in Hrel; rewrite nth_error_split in Hrel;
+            specialize (Hrel _ _ eq_refl).
+          destruct Hrel as [j Hj]; clarify.
+          destruct Hlocka; clarify.
+          * destruct (lt_dec j (length tr1)).
+            { specialize (Hacq (length tr1)); rewrite nth_error_split in Hacq.
+              specialize (Hacq _ _ eq_refl j u); clarify.
+              specialize (Hj22 x); use Hj22; [|omega].
+              specialize (Hj22 u); clarify. }
+            specialize (Hacq _ _ _ Hj21 (length tr1) t).
+            rewrite nth_error_app in Hj21; clarify.
+            use Hacq; [|destruct (eq_dec j (length tr1)); clarsimp; omega].
+            rewrite nth_error_split in Hacq; use Hacq.
+            destruct Hacq as [k Hk]; clarify.
+            rewrite nth_error_app in Hk2; destruct (lt_dec k (length tr1));
+              [omega|].
+            destruct (j - length tr1) as [|j'] eqn: Hminus; clarify.
+            destruct (k - length tr1) as [|k'] eqn: Hminus'; clarify.
+            rewrite nth_error_app in Hj21; destruct (lt_dec j' (length tr2));
+              [|omega].
+            generalize (nth_error_split' _ _ Hj21); intros [l0 [l3 ?]];
+              clarify.
+            rewrite <- app_assoc in Hk2; rewrite nth_error_app in Hk2;
+              destruct (lt_dec k' (length l0)); [|omega].
+            generalize (nth_error_split' _ _ Hk2); intros [l01 [l2 ?]]; clarify.
+            generalize (rtc_app_inv _ _ Hsteps2); intros [sc [Hsc ?]].
+            generalize (rtc_app_inv _ _ Hsc); intros [sr [? Hsr]].
+            inversion Hsr; clarify.
+            exists (acq t m :: l01), sr, s', l2, sc, (l3 ++ [rel u m]);
+              clarsimp.
+            split; [econstructor; eauto | clarify].
+            rewrite removelast_snoc; auto.
+          * rewrite nth_error_app in Hj21; destruct (lt_dec j (length tr1)).
+            { specialize (Hj22 (length tr1)); clarify.
+              rewrite nth_error_split in Hj22; specialize (Hj22 t);
+                contradiction Hj22; auto. }
+            destruct (j - length tr1) eqn: Hminus; clarify.
+            rewrite nth_error_app in Hj21; destruct (lt_dec n1 (length tr2));
+              [|omega].
+            generalize (nth_error_split' _ _ Hj21); intros [l2 [l3 ?]];
+              clarify.
+            generalize (rtc_app_inv _ _ Hsteps2); intros [sc [? Hsc]].
+            exists [], sa, sa', l2, sc, (l3 ++ [rel u m]); clarsimp.
+            split; [apply ss_refl | clarify].
+            rewrite removelast_snoc; auto. }
+      transitivity (K (rel t m) sr t t0); [|transitivity (K (acq u m) sc u t0)].
+      + destruct Hlocka; clarify.
+        * destruct l1; clarify.
+          inversion Hra21 as [|? ? ? ? Ha Hl1]; clarify.
+          generalize (clock_mono Hl1 t t0); inversion Ha; clarify.
+        * eapply clock_mono; eauto.
+      + simpl; unfold upd, vc_join; clarify.
+        generalize (rtc_snoc _ _ Hra21 Hra221); intro Hsteps.
+        generalize (rtc_trans Hsteps1 Hsteps); intro Hsteps'.
+        generalize (lock_mono Hsteps' Hra2221 m t0); intro Hlock.
+        etransitivity; [|apply Max.le_max_r].
+        etransitivity; [|apply Hlock].
+        inversion Hra221; clarify; unfold upd; clarify.
+        { assert ((tr1 ++ l1 ++ [rel t m]) ++ l2 =
+            firstn (length tr1 + length l1 + S (length l2))
+            (tr1 ++ a :: tr2 ++ b :: tr3)) as Heq.
+          { assert (a :: tr2 ++ b :: tr3 = (a :: tr2 ++ [b]) ++ tr3) as Heq
+              by clarsimp; rewrite Heq, Hra1; clarsimp.
+            rewrite <- plus_assoc, minus_plus; clarsimp.
+            rewrite firstn_length', firstn_length'; try omega.
+            rewrite not_le_minus_0; [|omega]; simpl; rewrite app_nil_r; auto. }
+          setoid_rewrite Heq; rewrite <- (firstn_skipn (length tr1 + length l1 +
+            S (length l2))) in Hfeasible; eapply feasible_app; eauto. }
+      + clarify.
+        destruct Hra2222 as [? | Hacq]; clarify.
+        * setoid_rewrite (split_app [] _ a) in Hra1;
+            rewrite (split_app l1), app_assoc, app_assoc in Hra1.
+          exploit app_inj_tail; eauto; clarify.
+        * inversion Hacq as [|? ? ? ? Hstep Hl3]; clarify.
+          generalize (clock_mono Hl3 u t0); inversion Hstep; clarify.
+          etransitivity; eauto.
+          unfold upd, vc_join in *; clarify.
+          apply Max.le_max_l.
+    - rewrite nth_error_split in Ha; clarify.
+      rewrite nth_error_app, lt_dec_plus_r, minus_plus in Hb; clarify.
+      rewrite nth_error_split in Hb; clarify.
+      destruct Ha0 as [? | Hfj]; [destruct Hb0 as [? | Hfj]; clarsimp|];
+        unfold fjs in *; destruct Hfj as [u Hfj].
+      + destruct Hfj; clarify.
+        * (* A thread doesn't act before it's forked. *)
+          inversion Hfeasible.
+          specialize (Hfork (length tr1 + S (length tr2)));
+            rewrite nth_error_app, lt_dec_plus_r, minus_plus in Hfork;
+            clarify; rewrite nth_error_split in Hfork.
+          specialize (Hfork _ _ eq_refl (length tr1) a);
+            rewrite nth_error_split in Hfork; clarify.
+          unfold uses_thread in Hfork.
+          use Hfork; [contradiction Hfork; clarify | omega].
+        * unfold upd, vc_join, vc_inc; clarify.
+          destruct (eq_dec (thread_of a) u); clarify.
+          etransitivity; [|apply Max.le_max_r].
+          etransitivity; [apply K_upper; eauto|].
+          eapply clock_mono; eauto.
+      + destruct Hfj; clarify; inversion Hstepa; clarify.
+        * destruct Hb0 as [? | Hfj]; clarify.
+          { generalize (clock_mono Hsteps2 (thread_of b) t0);
+              unfold upd, vc_join; clarify.
+            destruct (eq_dec u (thread_of b)); clarify.
+            etransitivity; [apply Max.le_max_r|].
+            etransitivity; [eauto | apply K_lower; auto]. }
+          destruct Hfj as [v [? | ?]]; clarify.
+          { (* A thread isn't forked twice. *)
+            inversion Hfeasible.
+            specialize (Hfork (length tr1 + S (length tr2)));
+              rewrite nth_error_app, lt_dec_plus_r, minus_plus in Hfork;
+              clarify; rewrite nth_error_split in Hfork.
+            specialize (Hfork _ _ eq_refl (length tr1) (fork u t));
+              rewrite nth_error_split in Hfork; clarify. 
+            use Hfork; [contradiction Hfork; clarify | omega].
+            unfold uses_thread, fjs; eauto. }
+          generalize (clock_mono Hsteps2 t t0).
+          unfold upd, vc_join, vc_inc; clarify.
+          destruct (eq_dec u t); clarify.
+          { generalize (fork_irrefl(t := t) (length tr1) Hfeasible);
+              rewrite nth_error_split; intro X; contradiction X; auto. }
+          destruct (eq_dec t v); clarify.
+          { generalize (join_irrefl(t := v) (length tr1 + S (length tr2))
+              Hfeasible); rewrite nth_error_app, lt_dec_plus_r, minus_plus;
+              simpl; rewrite nth_error_split; intro X; contradiction X; auto. }
+          etransitivity; [apply Max.le_max_r|].
+          etransitivity; eauto; apply Max.le_max_r.
+        * (* Nor does it act after it joins. *)
+          inversion Hfeasible.
+          specialize (Hjoin (length tr1)); rewrite nth_error_split in Hjoin.
+          specialize (Hjoin _ _ eq_refl (length tr1 + S (length tr2)));
+            rewrite nth_error_app, lt_dec_plus_r, minus_plus in Hjoin.
+          simpl in Hjoin; rewrite nth_error_split in Hjoin;
+            specialize (Hjoin b); use Hjoin; [clarify | omega].
+    - generalize (hb_lt Hhb1), (hb_lt Hhb2); intros Hlti Hltj.
+      destruct k; [omega | clarify].
+      rewrite <- plus_n_Sm in Hltj; rewrite <- Nat.succ_lt_mono in Hltj.
+      generalize (nth_error_succeeds tr2); intro Hk.
+      specialize (Hk (k - length tr1)); use Hk; [|omega].
+      destruct Hk as [c Hk].
+      generalize (nth_error_split' _ _ Hk); intros [l1 [l2 ?]]; clarify.
+      generalize (rtc_app_inv _ _ Hsteps2); intros [sc [Hl1 Hstepsc]].
+      inversion Hstepsc as [|? sc' ? ? Hstepc Hl2]; clarify.
+      transitivity (K c sc (thread_of c) t0).
+      + destruct (eq_dec (thread_of a) (thread_of c)).
+        { rewrite e; etransitivity; [apply K_upper; eauto|].
+          etransitivity; [|apply K_lower].
+          eapply clock_mono; eauto. }
+        eapply IHHhb1; eauto; clarsimp; omega.
+      + destruct (eq_dec (thread_of c) (thread_of b)).
+        { rewrite e; etransitivity; [apply K_upper; eauto|].
+          etransitivity; [|apply K_lower].
+          eapply clock_mono; eauto. }
+        generalize (ss_step _ _ Hstepa Hl1); intro Hstepsa.
+        generalize (rtc_trans Hsteps1 Hstepsa); intro.
+        eapply IHHhb2; eauto; clarsimp; omega.
+  Qed.
+
+  Lemma hb_clocks' sa a tr sb b : forall (Hwf : well_formed sa)
+    (Hsteps : step_star sa (a :: tr) sb) tr0 s (Hsteps0 : step_star s tr0 sa)
+    (Hfeasible : feasible (tr0 ++ a :: tr ++ [b]))
+    t (Ht : t = thread_of a) u (Hu : u = thread_of b)
+    (Hhb : happens_before (a :: tr ++ [b]) 0 (S (length tr)))
+    x (Ha : accesses a x) y (Hb : accesses b y),
+    vc_le (clock_of sa t) (clock_of sb u).
+  Proof.
+    intros.
+    inversion Hsteps as [|? ? ? ? Hstepa Htr]; clarify.
+    generalize (hb_app' tr0 Hhb); intro Hhb'; clarsimp.
+    generalize (hb_clocks Hsteps0 Hstepa Htr _ eq_refl eq_refl _ Hhb');
+      clarify.
+    destruct Ha as [? [? | ?]], Hb as [? [? | ?]]; clarify.
+  Qed.
+
+  Lemma no_writes : forall s tr s' x (Hsteps : step_star s tr s')
+    (Hno : Forall (fun a => ~writes a x) tr), write_of s' x = write_of s x.
+  Proof.
+    intros; induction Hsteps; clarify.
+    inversion Hno as [|? ? Ha ?]; clarify.
+    unfold writes in *; inversion Hstep; clarify.
+    unfold upd in *; clarify.
+    contradiction Ha; eauto.
+  Qed.
+
+  Opaque skipn.
+
+  Lemma access_write : forall tr s a x (Hsteps : step_star s0 tr s)
+    (Hrf : race_free' (tr ++ [a])) (Haccesses : accesses a x)
+    (Hfeasible : feasible (tr ++ [a])),
+    vc_le (write_of s x) (clock_of s (thread_of a)).
+  Proof.
+    intros.
+    destruct (last_write tr x) eqn: Hfind; clarify.
+    - unfold last_write in Hfind; rewrite find_index_spec in Hfind; clarify.
+      generalize (nth_error_rev' _ _ Hfind1); intro Hnth.
+      generalize (nth_error_lt _ _ Hnth); intro Hlt.
+      specialize (Hrf _ _ Hlt); rewrite nth_error_split, nth_error_app in Hrf;
+        clarify.
+      specialize (Hrf _ _ Hnth eq_refl x).
+      rewrite writesb_writes in Hfind21.
+      generalize (writes_accesses Hfind21); clarify.
+      rewrite <- (firstn_skipn (length tr - n - 1) tr) in Hrf at 1;
+        rewrite <- app_assoc in Hrf.
+      generalize (List.firstn_length (length tr - n - 1) tr);
+        rewrite Min.min_l; [intro Hlen | omega].
+      generalize (hb_suffix _ _ Hrf); setoid_rewrite Hlen; rewrite minus_diag.
+      rewrite <- (skipn_length (length tr - n - 1)); intro Hhb'; clarify.
+      rewrite <- (firstn_skipn (length tr - n - 1) tr) in Hsteps, Hfeasible.
+      erewrite skipn_n in Hsteps, Hfeasible, Hhb'; eauto.
+      erewrite (skipn_n (length tr - n - 1)) in Hhb'; eauto.
+      generalize (rtc_app_inv _ _ Hsteps); intros [s' [Hs' Hs]].
+      generalize (step_star_wf wf0 Hs'); intro Hwf'.
+      rewrite <- app_assoc in Hfeasible.
+      generalize (hb_clocks' Hwf' Hs Hs' Hfeasible eq_refl eq_refl Hhb' H
+        Haccesses); intro Hle.
+      intro; etransitivity; [|apply Hle].
+      destruct Hfind21 as [u ?]; subst.
+      inversion Hs as [|? ? ? ? Hstep Hnone]; clarify.
+      generalize (write_result Hstep); intros [Hw' Hc'].
+      generalize (rtc_snoc _ _ Hs' Hstep); intro Hs'0.
+      rewrite <- Hc' in *; generalize (write_own _ _ Hs'0 Hw'); intro Hle'.
+      etransitivity; [|apply Hle'].
+      erewrite no_writes; eauto.
+      rewrite Forall_forall; intros ? Hin.
+      generalize (in_nth_error _ _ Hin); intros [j Hj]; clarify.
+      rewrite skipn_length, skipn_nth in *.
+      rewrite <- writesb_writes, Bool.not_true_iff_false; eapply Hfind22;
+        [|apply nth_error_rev; eauto].
+      generalize (nth_error_lt _ _ Hfind1); rewrite rev_length; intro Hn.
+      clear - Hn Hj1; rewrite plus_comm, Nat.sub_add_distr,
+        (Nat.sub_succ_r (length tr)).
+      rewrite minus_distr, Nat.add_1_r; simpl; [| omega |].
+      rewrite minus_distr, minus_diag; [| omega | apply lt_le_weak; auto].
+      destruct n; omega.
+      { generalize (lt_not_le _ _ Hn); rewrite <- Nat.sub_0_le.
+        destruct (length tr - n) eqn: Hminus; setoid_rewrite Hminus;
+          [clarify | omega]. }
+    - unfold last_write in Hfind; rewrite find_index_fail in Hfind.
+      erewrite no_writes; eauto; [intro; clarify|].
+      rewrite Forall_rev in Hfind; eapply Forall_impl; eauto; clarify.
+      intro X; setoid_rewrite <- writesb_writes in X; clarify.
+  Qed.
+
+  Lemma read_step : forall s a s' tr s'' x t (Hstep : step s a s')
+    (Hwf : well_formed s) (Hsteps : step_star s' tr s'')
+    (Hle : vc_le (read_of s x) (clock_of s'' t))
+    (Hrf : accesses a x ->
+       happens_before (a :: tr ++ [wr t x]) 0 (S (length tr)))
+    tr0 s0 (Hsteps0 : step_star s0 tr0 s)
+    (Hfeasible : feasible (tr0 ++ a :: tr ++ [wr t x])),
+    vc_le (read_of s' x) (clock_of s'' t).
+  Proof.
+    intros; intro u.
+    inversion Hstep; clarify; unfold upd; clarify.
+    - assert (accesses (rd(lock := lock) t0 x) x) as Haccess
+        by (unfold accesses; eauto); clarify.
+      generalize (ss_step _ _ Hstep Hsteps); intro Hsteps'.
+      setoid_rewrite Nat.max_lub_iff; clarify.
+      assert (well_formed (C, L, R, W)) as Hwf by (split; auto).
+      generalize (hb_clocks' Hwf Hsteps' Hsteps0 Hfeasible eq_refl eq_refl Hrf
+        Haccess); intro Hle'; eapply Hle'.
+      unfold accesses; eauto.
+    - assert (accesses (wr(lock := lock) t0 x) x) as Haccess
+        by (unfold accesses; eauto); clarify.
+      generalize (ss_step _ _ Hstep Hsteps); intro Hsteps'.
+      assert (well_formed (C, L, R, W)) as Hwf by (split; auto).
+      generalize (hb_clocks' Hwf Hsteps' Hsteps0 Hfeasible eq_refl eq_refl Hrf
+        Haccess); intro Hle'; eapply Hle'.
+      unfold accesses; eauto.
+  Qed.
+
+  Lemma write_read_aux : forall tr s x t (Hsteps : step_star s0 tr s)
+    (Hread : forall tr1 sa a sa' tr2, tr = tr1 ++ a :: tr2 ->
+       step_star s0 tr1 sa -> step sa a sa' -> step_star sa' tr2 s ->
+       vc_le (read_of sa' x) (clock_of s t)),
+    vc_le (read_of s x) (clock_of s t).
+  Proof.
+    intros.
+    destruct (eq_dec tr []).
+    { subst; inversion Hsteps; intro; clarify. }
+    setoid_rewrite (app_removelast_last (wr t x)) in Hsteps; auto.
+    generalize (rtc_snoc_inv _ _ Hsteps); clarify.
+    eapply Hread; eauto; try (apply ss_refl).
+    apply app_removelast_last; auto.
+  Qed.
+
+  Lemma write_read : forall tr s t x (Hsteps : step_star s0 tr s)
+    (Hrf : forall i a, nth_error tr i = Some a -> accesses a x ->
+       happens_before (tr ++ [wr t x]) i (length tr))
+    (Hfeasible : feasible (tr ++ [wr t x])),
+    vc_le (read_of s x) (clock_of s t).
+  Proof.
+    intros; eapply write_read_aux; eauto.
+    induction tr1 using rev_ind; intros sa a sa' tr2 ? H0 Ha Htr2; clarify.
+    - inversion H0; clarify.
+      eapply read_step; eauto.
+      + apply wf0.
+      + intro; clarify.
+      + apply Hrf; auto.
+    - generalize (rtc_snoc_inv _ _ H0); intros [sx [Htr Hx]].
+      rewrite <- app_assoc in IHtr1; simpl in IHtr1;
+        specialize (IHtr1 _ _ _ _ eq_refl Htr Hx).
+      generalize (ss_step _ _ Ha Htr2); clarify.
+      eapply read_step; eauto.
+      + eapply (step_star_wf wf0); eauto.
+      + specialize (Hrf (length (tr1 ++ [x0])) a);
+          rewrite nth_error_split in Hrf; clarify.
+        rewrite (app_length (tr1 ++ [x0])) in Hrf.
+        rewrite <- app_assoc in Hrf; generalize (hb_suffix _ _ Hrf);
+          clarsimp.
+      + clarsimp.
+  Qed.
+
+  Theorem Completeness tr : feasible tr -> race_free tr ->
+    exists s, step_star s0 tr s.
+  Proof.
+    setoid_rewrite race_free_alt; induction tr using rev_ind;
+      intros Hfeasible Hrf.
+    { eexists; apply ss_refl. }
+    generalize (feasible_snoc _ _ Hfeasible); clarify.
+    generalize (rf_app _ _ Hrf); intro; use IHtr; destruct IHtr as [s Htr].
+    assert (exists s', step s x s') as [s' ?];
+      [|eexists; eapply rtc_snoc; eauto].
+    destruct s as (((C, L), R), W).
+    generalize (step_star_wf wf0 Htr); intro Hwf.
+    destruct x; try (eexists; econstructor; eauto; fail).
+    - eexists; eapply read_upd; eauto.
+      generalize (access_write(x := x) Htr Hrf); intro HW; clarify; apply HW;
+        unfold accesses; eauto.
+    - eexists; eapply write_upd; eauto.
+      + generalize (access_write(x := x) Htr Hrf); intro HW; clarify; apply HW;
+          unfold accesses; eauto.
+      + generalize (write_read(x := x) t Htr); intro HR; clarify; apply HR;
+          auto.
+        intros ? ? Hnth ?.
+        generalize (nth_error_lt _ _ Hnth); intro.
+        eapply Hrf; auto.
+        * rewrite nth_error_app; clarify; eauto 2.
+        * apply nth_error_split.
+        * unfold writes; eauto.
+        * unfold accesses; eauto.
+  Qed.
+
+  Theorem Correctness tr (Hfeasible : feasible tr) :
+    race_free tr <-> exists s, step_star s0 tr s.
+  Proof.
+    split.
+    - apply Completeness; auto.
+    - intros [? ?]; eapply Soundness; eauto.
+  Qed.
+
   (* Abstract Pure TSan *)
   Definition state := ((tid -> vector_clock) * (lock -> vector_clock) *
     (var -> list (tid * vector_clock)) *
@@ -32,44 +965,37 @@ Section TSan.
   | drop_keep t1 V1 Vs Vs' (Hnle : ~vc_le V1 V) (HVs : drop_le V Vs Vs') :
       drop_le V ((t1, V1) :: Vs) ((t1, V1) :: Vs').
 
-  Inductive step : state -> operation -> state -> Prop :=
+  Inductive TS_step : state -> operation -> state -> Prop :=
   | on_read : forall C L R W t x Vs' R'
      (HW : Forall (fun s => vc_le (snd s) (C t)) (W x))
      (HR : drop_le (C t) (R x) Vs') (HR' : R' = upd R x ((t, C t) :: Vs')),
-     step (C, L, R, W) (rd t x) (C, L, R', W)
+     TS_step (C, L, R, W) (rd t x) (C, L, R', W)
   | on_write : forall C L R W t x R' W'
      (* We must be able to drop all previous reads and writes *)
      (HR : Forall (fun s => vc_le (snd s) (C t)) (R x))
      (HW : Forall (fun s => vc_le (snd s) (C t)) (W x))
-     (HR' : R' = upd R x []) (HW' : W' = upd W x []),
-     step (C, L, R, W) (wr t x) (C, L, R', W')
+     (HR' : R' = upd R x [(t, C t)]) (HW' : W' = upd W x [(t, C t)]),
+     TS_step (C, L, R, W) (wr t x) (C, L, R', W')
   | on_signal : forall C L R W t m L' C' (HL' : L' = upd L m (C t))
       (HC' : C' = upd C t (vc_inc t (C t))),
-     step (C, L, R, W) (rel t m) (C', L', R, W)
+     TS_step (C, L, R, W) (rel t m) (C', L', R, W)
   | on_wait : forall C L R W t m C' (HC' : C' = upd C t (vc_join (C t) (L m))),
-     step (C, L, R, W) (acq t m) (C', L, R, W)
-(* Are fork and join handled by signal and wait?
-  | fork_step : forall C L R W t u C'
+     TS_step (C, L, R, W) (acq t m) (C', L, R, W)
+(* Are fork and join handled by signal and wait?*)
+  | on_fork : forall C L R W t u C'
       (HC' : C' = upd (upd C u (vc_join (C u) (C t))) t (vc_inc t (C t))),
-     step (C, L, R, W) (fork t u) (C', L, R, W)
-  | join_step : forall C L R W t u C'
+     TS_step (C, L, R, W) (fork t u) (C', L, R, W)
+  | on_join : forall C L R W t u C'
       (HC' : C' = upd (upd C t (vc_join (C t) (C u))) u (vc_inc u (C u))),
-     step (C, L, R, W) (join t u) (C', L, R, W)*).
+     TS_step (C, L, R, W) (join t u) (C', L, R, W).
 
-  Definition step_star := rtc step.
+  Definition TS_step_star := rtc TS_step.
 
-  Definition join_list (ss : list (tid * vector_clock)) :=
-    fold_left (fun V s => vc_join V (snd s)) ss vc_bot.
-
-  Lemma join_le_aux : forall V (ss : list (tid * vector_clock)) V0,
-    vc_le (fold_left (fun V s => vc_join V (snd s)) ss V0) V <->
-    vc_le V0 V /\ Forall (fun s => vc_le (snd s) V) ss.
-  Proof.
-    induction ss; clarify.
-    - split; clarify.
-    - rewrite IHss, vc_join_le; split; clarify.
-      inversion H2; clarify.
-  Qed.
+  Fixpoint join_list (ss : list (tid * vector_clock)) :=
+    match ss with
+    | [] => vc_bot
+    | (_, V) :: rest => vc_join V (join_list rest)
+    end.
 
   Lemma vc_bot_le : forall (V : vector_clock), vc_le vc_bot V.
   Proof. unfold vc_bot; repeat intro; omega. Qed.
@@ -78,7 +1004,11 @@ Section TSan.
   Lemma join_le : forall V ss, vc_le (join_list ss) V <->
     Forall (fun s => vc_le (snd s) V) ss.
   Proof.
-    intros; setoid_rewrite join_le_aux; split; clarify.
+    induction ss.
+    - split; clarify.
+    - destruct a; simpl.
+      rewrite vc_join_le, IHss; split; clarify.
+      inversion H; clarify.
   Qed.
 
   Definition finite (V : vector_clock) :=
@@ -118,38 +1048,204 @@ Section TSan.
 
   Definition TS_sim (s1 : VectorClocks.state) (s2 : state) := match s1, s2 with
     (C1, L1, R1, W1), (C2, L2, R2, W2) => C1 = C2 /\ L1 = L2 /\
-    forall x, join_list (R2 x) = R1 x /\ join_list (W2 x) = W1 x /\
-      Forall (fun s => finite (snd s)) (R2 x) /\
-      Forall (fun s => finite (snd s)) (W2 x) end.
+    (forall t, finite (C1 t)) /\ (forall m, finite (L1 m)) /\
+    forall x, vc_eq (join_list (R2 x)) (R1 x) /\
+              vc_eq (join_list (W2 x)) (W1 x) /\
+              Forall (fun s => finite (snd s)) (R2 x) /\
+              Forall (fun s => finite (snd s)) (W2 x) end.
+
+  Import RelationClasses.
+  Instance vc_eq_refl : Reflexive (@vc_eq tid).
+  Proof. repeat intro; auto. Qed.
+  Hint Resolve vc_eq_refl.
+
+  Instance vc_eq_trans : Transitive (@vc_eq tid).
+  Proof. repeat intro; etransitivity; eauto. Qed.
+
+  Instance vc_eq_sym : Symmetric (@vc_eq tid).
+  Proof. repeat intro; auto. Qed.
+
+  Instance vc_eq_eq : Equivalence (@vc_eq tid).
+  Proof.
+    constructor; [apply vc_eq_refl | apply vc_eq_sym | apply vc_eq_trans].
+  Qed.
+
+  Lemma finite_bot : finite vc_bot.
+  Proof.
+    exists []; clarify.
+  Qed.
+  Hint Resolve finite_bot.
+
+  Lemma finite_inc : forall V t, finite V -> finite (vc_inc t V).
+  Proof.
+    intros ??[??].
+    exists (t :: x); unfold vc_inc; clarify.
+    contradiction H0; auto.
+  Qed. 
+  Hint Resolve finite_inc.
 
   Lemma TS_sim0 : TS_sim (VectorClocks.s0) s0.
   Proof. clarify. Qed.
 
-  Definition VC_step_star := @VectorClocks.step_star _ _ _
-    tid_eq var_eq lock_eq.
+  Lemma vc_join_assoc : forall (V1 V2 V3 : vector_clock),
+    vc_eq (vc_join (vc_join V1 V2) V3) (vc_join V1 (vc_join V2 V3)).
+  Proof.
+    repeat intro; symmetry; apply Max.max_assoc.
+  Qed.
 
-  Lemma TS_sim1 : forall s1 tr s1' (Hsteps : VC_step_star s1 tr s1') s2
+  Lemma vc_join_sym : forall (V1 V2 : vector_clock),
+    vc_eq (vc_join V1 V2) (vc_join V2 V1).
+  Proof.
+    repeat intro; apply Max.max_comm.
+  Qed.
+
+  Import Morphisms.
+  Instance join_proper : Proper (vc_eq ==> vc_eq ==> vc_eq) (@vc_join tid).
+  Proof.
+    repeat intro; unfold vc_join; clarsimp.
+  Qed.
+
+  Lemma vc_absorb : forall (V V' : vector_clock), vc_le V V' ->
+    vc_eq (vc_join V V') V'.
+  Proof.
+    repeat intro; apply Max.max_r; auto.
+  Qed.
+
+  Lemma join_drop_le : forall V l l' (Hdrop : drop_le V l l'),
+    vc_eq (vc_join V (join_list l')) (vc_join (join_list l) V).
+  Proof.
+    intros; induction Hdrop; clarify.
+    - rewrite vc_join_sym; auto.
+    - rewrite IHHdrop, (vc_join_sym V1), vc_join_assoc, (vc_absorb Hle); auto.
+    - rewrite (vc_join_sym V1); rewrite <- vc_join_assoc, IHHdrop.
+      rewrite (vc_join_sym V1); repeat rewrite vc_join_assoc.
+      rewrite (vc_join_sym V); auto.
+  Qed.
+  
+  Instance vc_le_proper : Proper (vc_eq ==> vc_eq ==> iff) (@vc_le tid).
+  Proof.
+    repeat intro; split; repeat intro;
+      specialize (H1 t); rewrite H, H0 in *; auto.
+  Qed.
+
+  Lemma drop_finite : forall V l l' (Hdrop : drop_le V l l')
+    (Hfin : Forall (fun s => finite (snd s)) l),
+    Forall (fun s => finite (snd s)) l'.
+  Proof.
+    intros; induction Hdrop; clarify.
+    - inversion Hfin; clarify.
+    - inversion Hfin; clarify.
+  Qed.
+  Hint Resolve drop_finite.
+
+  Lemma drop_all : forall V Vs (Hle : Forall (fun s => vc_le (snd s) V) Vs),
+    drop_le V Vs [].
+  Proof.
+    induction Vs; intros.
+    - constructor.
+    - inversion Hle; clarify.
+      destruct a; constructor; auto.
+  Qed.
+
+  Lemma join_id_l : forall (V : vector_clock), vc_eq (vc_join vc_bot V) V.
+  Proof.
+    repeat intro; auto.
+  Qed.
+
+  Lemma join_id_r : forall (V : vector_clock), vc_eq (vc_join V vc_bot) V.
+  Proof.
+    repeat intro; setoid_rewrite Max.max_0_r; auto.
+  Qed.
+
+  Lemma finite_join : forall V V' (Hfin : finite V) (Hfin' : finite V'),
+    finite (vc_join V V').
+  Proof.
+    intros ?? [x Hfin] [x' Hfin'].
+    exists (x ++ x'); intros; rewrite in_app in *.
+    specialize (Hfin t); specialize (Hfin' t); unfold vc_join; clarsimp.
+  Qed.
+
+  Lemma TS_sim1 : forall s1 tr s1' (Hsteps : step_star s1 tr s1') s2
     (*tr0 (Hroot : VC_step_star s0 tr0 s1) s2 (Hwf : well_formed s2)*)
     (Hsim : TS_sim s1 s2),
-    exists s2', step_star s2 tr s2' /\ TS_sim s1' s2'.
+    exists s2', TS_step_star s2 tr s2' /\ TS_sim s1' s2'.
   Proof.
     intros ????; induction Hsteps; intros.
     { do 2 eexists; eauto; apply ss_refl. }
-    assert (exists s2', step s2 l s2' /\ TS_sim s' s2') as [s2' [Hstep' Hsim']].
+    assert (exists s2', TS_step s2 l s2' /\ TS_sim s' s2')
+      as [s2' [Hstep' Hsim']].
     destruct s2 as (((C2, L2), R2), W2).
     clear Hsteps IHHsteps; inversion Hstep; clarify.
-    - generalize (Hsim22 x); intros (Hr & Hw & Hfinr & Hfinw).
+    - generalize (Hsim2222 x); intros (Hr & Hw & Hfinr & Hfinw).
       rewrite <- Hw, join_le in HW.
       generalize (finite_drop (C2 t) Hfinr); intros [? Hdrop].
       do 2 eexists; [econstructor; eauto | unfold upd; clarify].
-
-(* Would it be safe to have the base algorithm write the whole VC instead of
-   just the current thread's time? *)
-      unfold join_list in *; simpl.
-
-  Lemma join_drop_le : forall t V l l' (Hdrop : drop_le V l l'),
-    join_list ((t, V) :: l') = vc_join 
-
-      unfold join_list; simpl
+      rewrite <- Hr; split; [apply join_drop_le|]; clarify.
+      constructor; eauto.
+    - generalize (Hsim2222 x); intros (Hr & Hw & Hfinr & Hfinw).
+      rewrite <- Hw, join_le in HW.
+      rewrite <- Hr, join_le in HR.
+      do 2 eexists; [econstructor; eauto | unfold upd; clarify].
+      rewrite join_id_r; clarify.
+      split; constructor; eauto.
+    - do 2 eexists; [econstructor; eauto | unfold upd; clarify].
+      apply finite_join; auto.
+    - do 2 eexists; [econstructor; eauto | unfold upd; clarify].
+      split; clarify.
+    - do 2 eexists; [econstructor; eauto | unfold upd; clarify].
+      apply finite_join; auto.
+    - do 2 eexists; [econstructor; eauto | unfold upd; clarify].
+      apply finite_join; auto.
     - specialize (IHHsteps _ Hsim'); clarify; do 2 eexists; eauto; econstructor;
         eauto.
+  Qed.
+
+  Lemma TS_sim2 : forall s2 tr s2' (Hsteps : TS_step_star s2 tr s2') s1
+    (*tr0 (Hroot : VC_step_star s0 tr0 s1) s2 (Hwf : well_formed s2)*)
+    (Hsim : TS_sim s1 s2),
+    exists s1', step_star s1 tr s1' /\ TS_sim s1' s2'.
+  Proof.
+    intros ????; induction Hsteps; intros.
+    { do 2 eexists; eauto; apply ss_refl. }
+    assert (exists s1', step s1 l s1' /\ TS_sim s1' s')
+      as [s1' [Hstep' Hsim']].
+    destruct s1 as (((C1, L1), R1), W1).
+    clear Hsteps IHHsteps; inversion Hstep; clarify.
+    - generalize (Hsim2222 x); intros (Hr & Hw & Hfinr & Hfinw).
+      rewrite <- join_le, Hw in HW.
+      do 2 eexists; [econstructor; eauto | unfold upd; clarify].
+      rewrite join_drop_le, Hr; clarify.
+      constructor; eauto.
+    - generalize (Hsim2222 x); intros (Hr & Hw & Hfinr & Hfinw).
+      rewrite <- join_le, Hw in HW.
+      rewrite <- join_le, Hr in HR.
+      do 2 eexists; [econstructor; eauto | unfold upd; clarify].
+      rewrite join_id_r; clarify.
+      split; constructor; eauto.
+    - do 2 eexists; [econstructor; eauto | unfold upd; clarify].
+      split; clarify.
+    - do 2 eexists; [econstructor; eauto | unfold upd; clarify].
+      apply finite_join; auto.
+    - do 2 eexists; [econstructor; eauto | unfold upd; clarify].
+      apply finite_join; auto.
+    - do 2 eexists; [econstructor; eauto | unfold upd; clarify].
+      apply finite_join; auto.
+    - specialize (IHHsteps _ Hsim'); clarify; do 2 eexists; eauto; econstructor;
+        eauto.
+  Qed.
+
+  Corollary TS_iff : forall tr, (exists s, TS_step_star s0 tr s) <->
+      exists s, step_star VectorClocks.s0 tr s.
+  Proof.
+    split; intros [s Hs].
+    - generalize (TS_sim2 Hs _ TS_sim0); clarify; eauto.
+    - generalize (TS_sim1 Hs _ TS_sim0); clarify; eauto.
+  Qed.
+
+  Theorem TS_Correctness tr (Hfeasible : feasible tr) :
+    race_free tr <-> exists s, TS_step_star s0 tr s.
+  Proof.
+    rewrite TS_iff; apply Correctness; auto.
+  Qed.
+
+End TSan.
